new definition for reaches

autth/PDA.lean
@@ -60,142 +60,127 @@ def stepSetN (n : ℕ) (R : Set (conf pda))  : Set (conf pda) :=
   | 0 => R
   | Nat.succ m => stepSet (stepSetN m R)
 
--- Martin: Could you use?
--- Stefan: I agree that an inductive definition like that of reaches' would be more natural.
-#check Relation.ReflTransGen
-inductive reaches' : conf pda → conf pda → Prop :=
-  | base : (r₁ : conf pda) → reaches' r₁ r₁
-  | step : {r₁ r' r₂ : conf pda} → (r'∈ step r₁) → (reaches' r' r₂) → reaches' r₁ r₂
 
-def reachesN (n : ℕ) (r₁ r₂ : conf pda) : Prop :=
-  r₂ ∈ stepSetN n {r₁}
+def Reaches₁ (r₁ r₂ : conf pda) : Prop := r₂ ∈ step r₁
+def Reaches : conf pda → conf pda → Prop := Relation.ReflTransGen Reaches₁
 
-def reaches (r₁ r₂ : conf pda) : Prop :=
-  ∃ n : ℕ, r₂ ∈ stepSetN n {r₁}
+inductive ReachesIn : ℕ → conf pda → conf pda → Prop :=
+  | refl : (r₁ : conf pda)  → ReachesIn 0 r₁ r₁
+  | step : {n: ℕ} → {r₁ r₂ r₃ : conf pda} → ReachesIn n r₁ r₂ → Reaches₁ r₂ r₃ → ReachesIn (n+1) r₁ r₃
 
 
 def acceptsByEmptyStack (pda : PDA Q T S) : Language T :=
   { w : List T | ∃ q : Q,
-      reaches (⟨pda.initial_state, w, [pda.start_symbol]⟩ : conf pda) ⟨q, [], []⟩ }
+      Reaches (⟨pda.initial_state, w, [pda.start_symbol]⟩ : conf pda) ⟨q, [], []⟩ }
 
 def acceptsByFinalState (pda : PDA Q T S) : Language T :=
   { w : List T | ∃ q  ∈ pda.final_states, ∃ γ : List S,
-      reaches (⟨pda.initial_state, w, [pda.start_symbol]⟩ : conf pda) ⟨q, [], γ⟩ }
+      Reaches (⟨pda.initial_state, w, [pda.start_symbol]⟩ : conf pda) ⟨q, [], γ⟩ }
 
 -- Martin: This theorem already exists.
 private theorem append_cancel (v x w : List T) : v ++ x = w ++ x ↔ v = w := by
   apply List.append_left_inj
 
 @[refl]
-theorem reaches_refl (r₁ : conf pda) : reaches r₁ r₁ := by
-  use 0; simp [stepSetN];
+theorem Reaches.refl (r₁ : conf pda) : Reaches r₁ r₁ := Relation.ReflTransGen.refl
+
+@[refl]
+theorem reachesIn.refl (r₁ : conf pda) : ReachesIn 0 r₁ r₁ := ReachesIn.refl r₁
 
 variable {r₁ r₂ : conf pda}
 
--- Martin: I have certain doubts about the usefullness of `reachesN` for your project.
-theorem reaches_iff_reachesN : reaches r₁ r₂ ↔ ∃ n : ℕ, reachesN n r₁ r₂ := by
-  simp only [reaches, reachesN]
 
-theorem reachesN_of_n_one {r₃ : conf pda} {n : ℕ} (h₁ : reachesN n r₁ r₂) (h₂ : reachesN 1 r₂ r₃) :
-    reachesN (n+1) r₁ r₃ := by
-  simp [reachesN, stepSetN, stepSet] at *
-  use r₂
+theorem reachesIn_zero (h: ReachesIn 0 r₁ r₂) : r₁ = r₂ := by
+  rcases h with _|_
+  · rfl
 
-theorem reachesN_one : reachesN 1 r₁ r₂ ↔ r₂ ∈ step r₁ := by
-  simp [reachesN,stepSetN,stepSet,stepSetN]
-
-theorem reachesN_iff_split_last {n : ℕ} :
-    (∃ c : conf pda, reachesN n r₁ c ∧ reachesN 1 c r₂) ↔ reachesN (n+1) r₁ r₂ := by
+theorem reaches₁_iff_reachesIn_one : Reaches₁ r₁ r₂ ↔ ReachesIn 1 r₁ r₂ := by
   constructor
-  · intro ⟨c, h⟩
-    exact reachesN_of_n_one h.1 h.2
+  · exact ReachesIn.step (by rfl)
   · intro h
-    simp [reachesN, stepSetN,stepSet] at h
-    obtain ⟨c, hc⟩ := h
-    use c
-    constructor
-    · rw [reachesN]
-      exact hc.1
-    · simp [reachesN,stepSet,stepSetN]
-      exact hc.2
+    rcases h with _ | ⟨h₁,h₂⟩
+    · apply reachesIn_zero at h₁
+      simp_all
 
-theorem reachesN_of_one_n {r₃ : conf pda} {n : ℕ} (h₁ : reachesN 1 r₁ r₂) (h₂ : reachesN n r₂ r₃) :
-    reachesN (n+1) r₁ r₃ := by
+theorem reachesIn_of_n_one {r₃ : conf pda} {n : ℕ} (h₁ : ReachesIn n r₁ r₂) (h₂ : ReachesIn 1 r₂ r₃) :
+    ReachesIn (n+1) r₁ r₃ :=  ReachesIn.step h₁ (reaches₁_iff_reachesIn_one.mpr h₂)
+
+
+theorem reachesIn_one : ReachesIn 1 r₁ r₂ ↔ r₂ ∈ step r₁ := by
+  rw [←reaches₁_iff_reachesIn_one,Reaches₁]
+
+theorem reachesIn_iff_split_last {n : ℕ} :
+    (∃ c : conf pda, ReachesIn n r₁ c ∧ ReachesIn 1 c r₂) ↔ ReachesIn (n+1) r₁ r₂ := by
+  constructor
+  · intro ⟨c,h⟩
+    exact reachesIn_of_n_one h.1 h.2
+  · intro h
+    rcases h with _ | @⟨n,_,c,_,h₀,h₁⟩
+    use c
+    exact ⟨h₀,reaches₁_iff_reachesIn_one.mp h₁⟩
+
+
+theorem reachesIn_of_one_n {r₃ : conf pda} {n : ℕ} (h₁ : ReachesIn 1 r₁ r₂) (h₂ : ReachesIn n r₂ r₃) :
+    ReachesIn (n+1) r₁ r₃ := by
   induction' n with n ih generalizing r₃
-  case zero =>
-    rw [reachesN,stepSetN] at h₂
-    apply Set.eq_of_mem_singleton at h₂
-    rw [h₂]
-    simp [h₁]
-  case succ =>
-    rw [←reachesN_iff_split_last] at h₂
-    obtain ⟨c,h₂⟩:=h₂
-    have := ih h₂.1
-    rw [←reachesN_iff_split_last]
-    use c
-    exact ⟨this,h₂.2⟩
+  · obtain ⟨rfl⟩ := reachesIn_zero h₂
+    simp_all
+  · obtain ⟨c,hc₁,hc₂⟩ := reachesIn_iff_split_last.mpr h₂
+    apply ReachesIn.step
+    exact ih hc₁
+    exact reaches₁_iff_reachesIn_one.mpr hc₂
 
-theorem reachesN_iff_split_first {n : ℕ}:
-    (∃ c : conf pda, reachesN 1 r₁ c ∧ reachesN n c r₂) ↔ reachesN (n+1) r₁ r₂ := by
+theorem reachesIn_iff_split_first {n : ℕ}:
+    (∃ c : conf pda, ReachesIn 1 r₁ c ∧ ReachesIn n c r₂) ↔ ReachesIn (n+1) r₁ r₂ := by
   constructor
-  · intro h
-    obtain ⟨c,h⟩ := h
-    apply reachesN_of_one_n h.1
-    exact h.2
+  · intro ⟨c,h₁,h₂⟩
+    exact reachesIn_of_one_n h₁ h₂
   · intro h
     induction' n with n ih generalizing r₂
-    case zero =>
-      use r₂
-      use h
-      dsimp [reachesN,stepSetN]
-      apply Set.mem_singleton
-    case succ =>
-      rw [←reachesN_iff_split_last] at h
-      obtain ⟨c',hc'⟩:= h
-      have := ih hc'.1
-      obtain ⟨c,hc⟩ := this
-      use c
-      use hc.1
-      apply reachesN_of_n_one hc.2
-      exact hc'.2
+    · use r₂
+    · rcases h with _|@⟨_,_,r₂',_,h₁,h₂⟩
+      obtain ⟨c,hc₁,hc₂⟩ := ih h₁
+      refine ⟨c,hc₁,?_⟩
+      apply reachesIn_of_n_one
+      exact hc₂
+      exact reaches₁_iff_reachesIn_one.mp h₂
 
-theorem reachesN_trans {r₃ : conf pda} {n m : ℕ} (h₁ : reachesN n r₁ r₂) (h₂ : reachesN m r₂ r₃) :
-    ∃ k ≤ n+m, reachesN k r₁ r₃ := by
+
+theorem ReachesIn.trans {r₃ : conf pda} {n m : ℕ} (h₁ : ReachesIn n r₁ r₂) (h₂ : ReachesIn m r₂ r₃) :
+    ∃ k ≤ n+m, ReachesIn k r₁ r₃ := by
   induction' m with m ih generalizing r₃
-  · simp [reachesN,stepSetN] at h₂
-    rw [←h₂] at h₁
-    use n
-    refine ⟨?_, h₁⟩
-    linarith
-  · rw [reachesN,stepSetN,stepSet] at h₂
-    simp at h₂
-    obtain ⟨c,h⟩ :=  h₂
-    have r₂_reaches_c: reachesN m r₂ c := by
-      simp [reachesN, stepSetN, stepSet] at *
-      exact h.1
-    apply ih at r₂_reaches_c
-    have c_reaches_r₃ : reachesN 1 c r₃ := by
-      simp [reachesN, stepSetN, stepSet] at *
-      exact h.2
-    obtain ⟨k,h⟩ := r₂_reaches_c
+  · use n
+    apply reachesIn_zero at h₂
+    simp_all
+  · obtain ⟨c,hc₁,hc₂⟩:= reachesIn_iff_split_last.mpr h₂
+    obtain ⟨k,ih⟩ := ih hc₁
     use k+1
-    constructor
-    linarith
-    exact reachesN_of_n_one h.2 c_reaches_r₃
+    exact ⟨by linarith [ih.1],reachesIn_iff_split_last.mp ⟨c, ih.2, hc₂⟩⟩
 
-theorem reaches_trans {r₃ : conf pda} (h₁ : reaches r₁ r₂) (h₂ : reaches r₂ r₃) :
-    reaches r₁ r₃ := by
-  rw [reaches] at *
-  obtain ⟨n,hn⟩ := h₁
-  obtain ⟨m,hm⟩ := h₂
-  rw [←reachesN] at *
-  obtain ⟨k,hk⟩ := reachesN_trans hn hm
-  use k
-  exact hk.2
+theorem reaches_iff_reachesIn : Reaches r₁ r₂ ↔ ∃ n : ℕ, ReachesIn n r₁ r₂ := by
+  constructor
+  · intro h
+    induction h with
+    | refl => use 0
+    | @tail c r₂ h₁ h₂ ih =>
+      obtain ⟨n,hn⟩ := ih
+      use n+1
+      rw [←reachesIn_iff_split_last]
+      exact ⟨c, hn, reaches₁_iff_reachesIn_one.mp h₂⟩
+  · intro ⟨n,hn⟩
+    induction' n with n ih generalizing r₂
+    · apply reachesIn_zero at hn
+      rw [hn]
+    · obtain ⟨c,hc₁,hc₂⟩ :=  reachesIn_iff_split_last.mpr hn
+      rw [←reaches₁_iff_reachesIn_one] at hc₂
+      exact Relation.ReflTransGen.tail (ih hc₁) hc₂
 
-theorem decreasing_input_one (h : reachesN 1 r₁ r₂) :
+theorem Reaches.trans {r₃ : conf pda} (h₁ : Reaches r₁ r₂) (h₂ : Reaches r₂ r₃) :
+    Reaches r₁ r₃ := Relation.ReflTransGen.trans h₁ h₂
+
+theorem decreasing_input_one (h : ReachesIn 1 r₁ r₂) :
     ∃ w : List T, r₁.input = w ++ r₂.input := by
-  apply reachesN_one.mp at h
+  apply reachesIn_one.mp at h
   rcases r₁ with ⟨q,_|⟨a,w⟩,_|⟨Z,β⟩⟩ <;> simp [PDA,conf,step] at *
   · rw [h]
   · obtain ⟨_,_,h⟩ := h
@@ -212,17 +197,15 @@ theorem decreasing_input_one (h : reachesN 1 r₁ r₂) :
       rw [h.2]
       simp
 
-theorem decreasing_input (h : reaches r₁ r₂) :
+theorem decreasing_input (h : Reaches r₁ r₂) :
     ∃ w : List T, r₁.input = w ++ r₂.input := by
-  rw [reaches] at h
+  rw [reaches_iff_reachesIn] at h
   obtain ⟨n,h'⟩ := h
-  rw [←reachesN] at h'
   induction' n with n ih generalizing r₂
-  · simp [reachesN, stepSetN, stepSet, step] at h'
+  · apply reachesIn_zero at h'
     use []
-    rw [h']
-    simp
-  · apply reachesN_iff_split_last.mpr at h'
+    simp_all
+  · apply reachesIn_iff_split_last.mpr at h'
     obtain ⟨c,h',h''⟩ := h'
     apply ih at h'
     apply decreasing_input_one at h''
@@ -232,19 +215,14 @@ theorem decreasing_input (h : reaches r₁ r₂) :
     simp [hw₁,hw₂]
 
 theorem unconsumed_input_one (x : List T) :
-    reachesN 1 r₁ r₂ ↔ reachesN 1 (r₁.appendInput x) (r₂.appendInput x) := by
+    ReachesIn 1 r₁ r₂ ↔ ReachesIn 1 (r₁.appendInput x) (r₂.appendInput x) := by
   constructor
   · intro h
     rcases r₂ with ⟨p,v,α⟩
     rcases r₁ with ⟨q,_|⟨a,w⟩,_|⟨Z,β⟩⟩ <;>
-    simp [reachesN,conf.appendInput,stepSetN,stepSet,step] at *
+    simp [reachesIn_one,step,conf.appendInput] at *
     · assumption
-    · rcases x with _|⟨a,w⟩
-      · simp
-        exact h
-      · simp
-        right
-        exact h
+    · rcases x with _|⟨a,w⟩ <;> simp_all
     · simp [h]
     · rw [←List.cons_append]
       rw [append_cancel]
@@ -252,7 +230,7 @@ theorem unconsumed_input_one (x : List T) :
   · intro h
     rcases r₂ with ⟨p,v,α⟩
     rcases r₁ with ⟨q,_|⟨a,w⟩,_|⟨Z,β⟩⟩ <;>
-    simp [reachesN,conf.appendInput,stepSetN,stepSet,step] at *
+    simp [reachesIn_one,step,conf.appendInput] at *
     · assumption
     · rcases x with _|⟨a,w⟩
       · simp at h; assumption
@@ -267,29 +245,30 @@ theorem unconsumed_input_one (x : List T) :
     · rwa [←List.cons_append, append_cancel] at h
 
 theorem unconsumed_input_N {n : ℕ} (x : List T) :
-    reachesN n r₁ r₂ ↔ reachesN n (r₁.appendInput x) (r₂.appendInput x) := by
+    ReachesIn n r₁ r₂ ↔ ReachesIn n (r₁.appendInput x) (r₂.appendInput x) := by
   constructor
   · induction' n with n ih generalizing r₁ r₂
     case zero =>
       intro h
-      simp [reachesN,stepSetN] at h
+      apply reachesIn_zero at h
       rw [h]
-      simp [reachesN, stepSetN]
     case succ =>
       intro h
-      apply reachesN_iff_split_last.mpr at h
+      apply reachesIn_iff_split_last.mpr at h
       obtain ⟨c,h'⟩ := h
-      have : reachesN n (r₁.appendInput x) (c.appendInput x) := ih h'.1
+      have : ReachesIn n (r₁.appendInput x) (c.appendInput x) := ih h'.1
       apply And.right at h'
       rw [unconsumed_input_one x] at h'
-      rw [←reachesN_iff_split_last]
+      rw [←reachesIn_iff_split_last]
       use c.appendInput x
   · induction' n with n ih generalizing r₁ r₂
-    · simp [reachesN, stepSetN]
-      intros
-      ext <;> aesop
     · intro h
-      rw [←reachesN_iff_split_last] at *
+      apply reachesIn_zero at h
+      simp only [conf.appendInput,conf.mk.injEq] at h
+      obtain rfl : r₁ = r₂ := by ext <;> simp_all
+      rfl
+    · intro h
+      rw [←reachesIn_iff_split_last] at *
       obtain ⟨c,h⟩ := h
       have := decreasing_input_one h.2
       obtain ⟨w,h'⟩ := this
@@ -307,201 +286,45 @@ theorem unconsumed_input_N {n : ℕ} (x : List T) :
         exact h.2
 
 theorem unconsumed_input (x : List T) :
-    reaches r₁ r₂ ↔ reaches (r₁.appendInput x) (r₂.appendInput x) := by
+    Reaches r₁ r₂ ↔ Reaches (r₁.appendInput x) (r₂.appendInput x) := by
+  rw [reaches_iff_reachesIn,reaches_iff_reachesIn]
   constructor <;> intro ⟨n,h'⟩ <;> use n
   · exact (unconsumed_input_N x).mp h'
   · exact (unconsumed_input_N x).mpr h'
 
-theorem reachesN_one_iff : reachesN 1 r₁ r₂ ↔
-     ∃ c : ℕ → conf pda, reachesN 1 r₁ (c 0) ∧
-      (∀ i < 0, reachesN 1 (c i) (c i.succ)) ∧ c 0 = r₂ := by
-  constructor
-  · intro h
-    use λ_↦r₂
-    simpa
-  · intro h
-    obtain ⟨c, hr, -, hc⟩:= h
-    convert hr
-    exact hc.symm
 
-theorem reachesN_iff {n : ℕ} (hn : 0 < n) : reachesN n r₁ r₂ ↔
-    ∃ c : ℕ → conf pda, reachesN 1 r₁ (c 0) ∧
-      (∀ i < n - 1, reachesN 1 (c i) (c i.succ)) ∧ c (n-1) = r₂ := by
-  constructor
-  · rcases n with _|⟨n⟩
-    case zero => contradiction
-    case succ =>
-      induction' n with n ih generalizing r₂
-      case zero =>
-        intro h
-        rw [reachesN_one_iff] at h
-        tauto
-      case succ =>
-        simp
-        intro h
-        rw [←reachesN_iff_split_last] at h
-        obtain ⟨cₙ,h₁,h₂⟩ := h
-        apply ih (Nat.zero_lt_succ n) at h₁
-        obtain ⟨c₀,h₀⟩ := h₁
-        simp at h₀
-        set c := λm↦if m < n+1 then c₀ m else r₂
-        refine ⟨c, ?_,?_,?_⟩
-        · simp [c, hn, h₀]
-        · intro i hi
-          by_cases hin : i=n <;> simp [c, hin,hi]
-          · simp [h₀,h₂]
-          · apply Nat.le_of_lt_succ at hi
-            have := lt_iff_le_and_ne.mpr (And.intro hi hin)
-            simp [this]
-            exact h₀.2.1 i this
-        · simp [c]
-  · rcases n with _|⟨n⟩
-    case zero => contradiction
-    case succ =>
-      induction' n with n ih generalizing r₂
-      case zero =>
-        rw [reachesN_one_iff]
-        tauto
-      case succ =>
-        intro h
-        simp at h
-        obtain ⟨c,h'⟩ := h
-        have : reachesN (n+1) r₁ (c n) := by
-          apply ih
-          · linarith
-          refine ⟨c, ?_,?_,?_⟩
-          · tauto
-          · intro i hi
-            have : i<n+1 := by simp at hi; linarith
-            apply h'.2.1 i this
-          · simp
-        have cₙr₂ : reachesN 1 (c n) r₂ := by
-          rw [←h'.2.2]
-          apply h'.2.1
-          norm_num
-        apply reachesN_of_n_one
-        exact this
-        exact cₙr₂
-
-theorem reachesN_zero : reachesN 0 r₁ r₂ ↔ r₁ = r₂ := by
-  constructor
-  · rw [reachesN,stepSetN,Set.mem_singleton_iff]
-    exact Eq.symm
-  · intro h
-    simp [h, reachesN, stepSetN]
-
-theorem reachesN_pos_of_not_self {n : ℕ} (h : r₁ ≠ r₂) :
-    reachesN n r₁ r₂ → n > 0 := by
+theorem reachesIn_pos_of_not_self {n : ℕ} (h : r₁ ≠ r₂) :
+    ReachesIn n r₁ r₂ → n > 0 := by
   rcases n with _ | ⟨n⟩
   · intro h
-    apply reachesN_zero.mp at h
+    apply reachesIn_zero at h
     contradiction
   · intro _
     apply Nat.zero_lt_succ
 
-theorem reaches_iff (h : r₁ ≠ r₂) : reaches r₁ r₂ ↔
-    ∃ (n : ℕ) (c : ℕ → conf pda), reachesN 1 r₁ (c 0) ∧
-      (∀ i < n, reachesN 1 (c i) (c i.succ)) ∧ c n = r₂ := by
-  constructor
-  · intro h
-    rw [reaches] at h
-    obtain ⟨n,h'⟩ := h
-    rw [←reachesN] at h'
-    have n_pos : n>0 := reachesN_pos_of_not_self h h'
-    rw [reachesN_iff n_pos] at h'
-    obtain ⟨c,h''⟩ := h'
-    use n-1, c
-  · intro ⟨n,hn⟩
-    set m := n+1 with m_def
-    have m_pos : m>0 := by linarith
-    rw [show n = m-1 by simp [m_def]] at hn
-    rw [←reachesN_iff m_pos] at hn
-    rw [reaches]
-    use m
-    rwa [←reachesN]
-
-theorem unconsumed_stack_one (hr₁s : r₁.stack ≠ []) (γ : List S) :
-    reachesN 1 r₁ r₂ ↔ reachesN 1 (r₁.appendStack γ) (r₂.appendStack γ) := by
-  rcases r₁ with ⟨q,x,α⟩
-  rcases r₂ with ⟨p,y,β⟩
-  constructor
-  <;> intro h
-  <;> rw [reachesN_one] at *
-  <;> simp [conf.appendStack] at *
-  <;> rcases x with _|⟨a,w⟩
-  <;> rcases α with _|⟨Z,ν⟩
-  <;> rcases γ with _|⟨X,μ⟩
-  <;> simp [step] at *
-  <;> try assumption
-  · obtain ⟨p₁, beta₁, h'⟩ := h
-    use p₁, beta₁
-    simp [h']
-  · rcases h with h|h
-    · left
-      obtain ⟨p₁, beta₁, h'⟩ := h
-      use p₁, beta₁
-      simp [h']
-    · right
-      obtain ⟨p₁, beta₁, h'⟩ := h
-      use p₁, beta₁
-      simp [h']
-  · rw [List.append_cons, List.append_cons ν X μ] at h
-    obtain ⟨p₁, β₁, h'⟩ := h
-    use p₁, β₁
-    simp [h' ]
-    have : β ++ ([X] ++ μ) = (β₁ ++ ν) ++ ([X] ++ μ) := by
-      have := h'.2.2.2
-      rw [←List.append_assoc,this]
-      simp
-    rwa [append_cancel] at this
-  · rcases h with ⟨p₁,β₁,h'⟩|⟨p₁,β₁,h'⟩
-    · left
-      use p₁, β₁
-      use h'.1, h'.2.1, h'.2.2.1
-      have : β ++ ([X] ++ μ) = (β₁ ++ ν) ++ ([X] ++ μ) := by
-        rw [List.append_cons _ X μ] at h'
-        rw [←List.append_assoc, h'.2.2.2]
-        simp
-      rwa [append_cancel] at this
-    · right
-      use p₁, β₁
-      use h'.1, h'.2.1, h'.2.2.1
-      have : β ++ ([X] ++ μ) = (β₁ ++ ν) ++ ([X] ++ μ) := by
-        repeat rw [List.append_cons _ X μ] at h'
-        rw [←List.append_assoc, h'.2.2.2]
-        simp
-      rwa [append_cancel] at this
-
-theorem unconsumed_stackN {n : ℕ} (hr₁s : r₁.stack ≠ []) (hr₂s : r₂.stack ≠ [])
-    (γ : List S) :
-  reachesN n r₁ r₂ ↔
-    ∃ c : ℕ → conf pda, reachesN 1 (r₁.appendStack γ) (c 0) ∧
-      (∀ i < n, (c i).stackPostfix γ) ∧
-      (∀ i < n - 1, reachesN 1 (c i) (c i.succ)) ∧ c (n-1) = r₂.appendStack γ := by sorry
-
-theorem reachesN_one_on_empty_stack {q p: Q}{w w': List T}{α : List S}:
-    pda.reachesN 1 ⟨q, w, []⟩ ⟨p, w', α⟩ → w=w' ∧ α = [] ∧ q=p:= by
+theorem reachesIn_one_on_empty_stack {q p: Q}{w w': List T}{α : List S}:
+    pda.ReachesIn 1 ⟨q, w, []⟩ ⟨p, w', α⟩ → w=w' ∧ α = [] ∧ q=p:= by
   intro h
-  rw [reachesN_one] at h
+  rw [reachesIn_one] at h
   simp only [step] at h
   rw [Set.mem_setOf, conf.mk.injEq] at h
   simp [h]
 
 theorem reaches_on_empty_stack {q p: Q}{w w': List T}{α : List S}:
-    pda.reaches ⟨q, w, []⟩ ⟨p, w', α⟩ → w=w' ∧ α = [] := by
+    pda.Reaches ⟨q, w, []⟩ ⟨p, w', α⟩ → w=w' ∧ α = [] := by
   intro h
-  rw [reaches_iff_reachesN] at h
+  rw [reaches_iff_reachesIn] at h
   obtain ⟨n,hr⟩ := h
   induction' n with n ih
-  · rw [reachesN_zero,conf.mk.injEq] at hr
+  · apply reachesIn_zero at hr
+    rw [conf.mk.injEq] at hr
     simp [hr]
-  · rw [←reachesN_iff_split_first] at hr
+  · rw [←reachesIn_iff_split_first] at hr
     obtain ⟨⟨q',v,α'⟩,h₁,h₂⟩ := hr
-    apply reachesN_one_on_empty_stack at h₁
+    apply reachesIn_one_on_empty_stack at h₁
     rw  [←h₁.1, h₁.2.1, ←h₁.2.2] at h₂
     apply ih at h₂
     simp [h₂]
 
-theorem reaches_of_reachesN  {n: ℕ}(h: pda.reachesN n r₁ r₂) : pda.reaches r₁ r₂ := by
-  rw [reaches_iff_reachesN]
-  use n
+theorem reaches_of_reachesIn  {n: ℕ}(h: pda.ReachesIn n r₁ r₂) : pda.Reaches r₁ r₂ :=
+  reaches_iff_reachesIn.mpr ⟨n, h⟩
